src/Lifetime.v
@@ -85,7 +85,7 @@ Proof.
   - specialize (H l). specialize (H0 l). etransitivity; eauto.
 Qed.
 
-Lemma Lifetimes_lte_cons ls ls' a a' :
+Lemma Lifetimes_lte_cons_inv ls ls' a a' :
   Lifetimes_lte (a :: ls) (a' :: ls') ->
   Lifetimes_lte ls ls'.
 Proof.
@@ -101,7 +101,7 @@ Proof.
   destruct ls'.
   - specialize (H 0). contradiction.
   - cbn. apply le_n_S. apply IHls.
-    eapply Lifetimes_lte_cons; eauto.
+    eapply Lifetimes_lte_cons_inv; eauto.
 Qed.
 
 Lemma Lifetimes_lte_app ls ls' r :
@@ -132,6 +132,20 @@ Proof.
       * erewrite nth_error_replace_list_index_neq_new; try lia.
         destruct (nth_error ls l'); [destruct s |]; cbn; auto.
 Qed.
+
+Lemma Lifetimes_lte_replace_list_index_inv ls ls' l s :
+  Lifetimes_lte (replace_list_index ls l s) (replace_list_index ls' l s) ->
+  statusOf_lte (statusOf l ls) (statusOf l ls') ->
+  Lifetimes_lte ls ls'.
+Proof.
+  intros Hreplace Hl l'. specialize (Hreplace l').
+  destruct (Compare_dec.lt_eq_lt_dec l l') as [[? | ?] | ?]; subst; auto.
+
+  (* destruct (Peano_dec.dec_eq_nat l l'); subst; auto. *)
+  destruct (Compare_dec.dec_lt l (length ls)).
+  -
+    destruct (Compare_dec.dec_lt l (length ls')).
+Admitted.
 
 Lemma Lifetimes_lte_replace_list_index ls ls' l s :
   Lifetimes_lte ls ls' ->
